Add some features to the pretty printer
The output of the pretty printer is now legible: boolean operators are
printed infix, binder notation for !/?/?!/@ is supported, and negations
(~) are printed properly. Also adds some PMATCH definitions.

candle/standard/opentheory/prettyScript.sml
@@ -1,5 +1,4 @@
 open preamble holSyntaxTheory mlstringTheory
-     NumProgTheory (* cannot load mlnumTheory? *)
 
 val _ = new_theory "pretty";
 
@@ -147,23 +146,27 @@ val name_of_def = Define `
     else if nm = strlit"Data.Bool.F" then
       strlit"F"
     else if nm = strlit"Data.Bool.cond" then
-      strlit"COND"
+      strlit"cond"
     else
       nm`;
 
 val is_binop_def = Define `
-  is_binop con tm =
+  is_binop tm =
     case tm of
-      Comb (Comb (Const con' _) _) _ => con = con'
+      Comb (Comb (Const con _) _) _ =>
+        (case fixity_of con of
+           right _ => T
+         | _ => F)
     | _ => F`;
 
 val is_binder_def = Define `
   is_binder tm =
     case tm of
-      Comb (Const nm _) (Abs _ _) =>
+      Comb (Const nm _) (Abs (Var _ _) _) =>
         nm = strlit"Data.Bool.?" \/
         nm = strlit"Data.Bool.!" \/
-        nm = strlit"Data.Bool.?!"
+        nm = strlit"Data.Bool.?!" \/
+        nm = strlit"@"
     | _ => F`;
 
 val is_cond_def = Define `
@@ -173,9 +176,11 @@ val is_cond_def = Define `
         con = strlit"Data.Bool.cond"
     | _ => F`;
 
-(* TODO
- * - add destructors for NUMERALs, lists of things, and binary operations
- *   (all of these are simply special cases of Comb). *)
+val is_neg_def = Define `
+  is_neg tm =
+    case tm of
+      Comb (Const nm _) _ => nm = strlit"Data.Bool.~"
+    | _ => F`;
 
 val collect_vars_def = Define `
   collect_vars tm =
@@ -193,6 +198,66 @@ val collect_vars_term_size = Q.store_thm("collect_vars_term_size",
   \\ TRY pairarg_tac \\ fs []
   \\ rw [term_size_def]);
 
+val dest_binary_def = Define `
+  dest_binary nm tm =
+    case tm of
+      Comb (Comb (Const nm' _) l) r =>
+        if nm <> nm' then
+          ([], tm)
+        else
+          let (ls, r) = dest_binary nm r in
+            (l::ls, r)
+    | _ => ([], tm)`;
+
+val dest_binary_term_size = Q.store_thm("dest_binary_term_size",
+  `term_size (SND (dest_binary nm tm)) <= term_size tm`,
+  Induct_on `tm`
+  \\ rw [Once dest_binary_def, term_size_def]
+  \\ PURE_CASE_TAC \\ fs [] \\ rw [term_size_def]
+  \\ PURE_CASE_TAC \\ fs [] \\ rw [term_size_def]
+  \\ fs [UNCURRY]);
+
+val dest_binary_MEM_term_size = Q.store_thm("dest_binary_MEM_term_size",
+  `!nm tm ts t q.
+     MEM t ts /\
+     dest_binary nm tm = (ts, q)
+     ==>
+     term_size t < term_size tm`,
+  recInduct (theorem "dest_binary_ind")
+  \\ rpt gen_tac \\ strip_tac
+  \\ Induct
+  \\ rw [Once dest_binary_def]
+  \\ pop_assum mp_tac
+  \\ PURE_TOP_CASE_TAC \\ fs []
+  \\ PURE_TOP_CASE_TAC \\ fs []
+  \\ PURE_TOP_CASE_TAC \\ fs []
+  \\ rw []
+  \\ pairarg_tac \\ fs [] \\ rw []
+  \\ rw [term_size_def]
+  \\ res_tac \\ fs []);
+
+val dest_binder_def = Define `
+  dest_binder nm tm =
+    case tm of
+      Comb (Const nm' _) (Abs (Var v _) b) =>
+        if nm <> nm' then
+          ([], tm)
+        else
+          let (vs, r) = dest_binder nm b in
+            (v::vs, r)
+    | _ => ([], tm)`;
+
+val dest_binder_term_size = Q.store_thm("dest_binder_term_size",
+  `!nm tm vs b. dest_binder nm tm = (vs, b) ==> term_size b <= term_size tm`,
+  recInduct (theorem "dest_binder_ind")
+  \\ rw []
+  \\ pop_assum mp_tac
+  \\ simp [Once dest_binder_def]
+  \\ rpt (PURE_TOP_CASE_TAC \\ fs [])
+  \\ pairarg_tac
+  \\ rw [term_size_def]
+  \\ fs []);
+
 (* ------------------------------------------------------------------------- *)
 (* A pretty printer for terms.                                               *)
 (* ------------------------------------------------------------------------- *)
@@ -207,18 +272,50 @@ val pp_paren_blk_def = Define `
 val pp_seq_def = Define `
   pp_seq pf brk sep ts =
     case ts of
-      [] => []
+      []    => []
+    | [t]   => [pf t]
     | t::ts =>
         pf t  ::
         mk_str sep ::
         if brk then [mk_brk 1] else [] ++
         pp_seq pf brk sep ts`;
 
+val interleave_def = Define `
+  interleave sep ts =
+    case ts of
+      []    => []
+    | [t]   => [t]
+    | t::ts => t::mk_str sep::mk_brk 1::interleave sep ts`;
+
 val pp_term_def = tDefine "pp_term" `
   (pp_term (prec: num) tm =
     case tm of
       Comb l r =>
-        if is_cond tm then
+        if is_neg tm then
+          pp_paren_blk 0 (prec = 1000) [pp_term 999 l; pp_term 1000 r]
+        else if is_binop tm then
+          (case l of
+             Comb (Const nm _) l =>
+               (case dest_binary nm tm of
+                  ([], _) => mk_str (strlit"<pp_term: bogus BINOP>")
+               | (tms, tmt) =>
+                   let args = tms ++ [tmt] in
+                   let sep  = space ^ name_of nm in
+                     (case fixity_of nm of
+                        left _ => mk_str (strlit"<pp_term: bogus BINOP>")
+                      | right nprec =>
+                          let ts = MAP (pp_term nprec) args in
+                            pp_paren_blk
+                              (if nprec <= prec then 1 else 0)
+                              (nprec <= prec)
+                              (interleave sep ts))
+           | _ =>
+             pp_paren_blk 0
+                 (prec = 1000)
+                 [pp_term 999 l;
+                  mk_brk 1;
+                  pp_term 1000 r]))
+        else if is_cond tm then
           (case l of
             Comb (Comb c p) l =>
               pp_paren_blk 0 (0 < prec)
@@ -230,7 +327,28 @@ val pp_term_def = tDefine "pp_term" `
                  mk_brk 1;
                  mk_str (strlit"else ");
                  pp_term 0 r]
-          | _ => mk_str (strlit"<pp_term: bogus COND>"))
+          | _ =>
+             pp_paren_blk 0
+                 (prec = 1000)
+                 [pp_term 999 l;
+                  mk_brk 1;
+                  pp_term 1000 r])
+        else if is_binder tm then
+          (case tm of
+            Comb (Const nm _) (Abs (Var v _) b) =>
+              let (vs, b) = dest_binder nm tm in
+              let ind = if prec = 0 then 4 else 5 in
+                pp_paren_blk ind (0 < prec)
+                  ((mk_str (name_of nm) :: pp_seq mk_str F space vs) ++
+                   [mk_str (strlit".");
+                    (if 1 < LENGTH vs then mk_brk 1 else mk_str space);
+                    pp_term 0 b])
+           | _ =>
+               pp_paren_blk 0
+                 (prec = 1000)
+                 [pp_term 999 l;
+                  mk_brk 1;
+                  pp_term 1000 r])
         else
           pp_paren_blk 0
             (prec = 1000)
@@ -238,28 +356,29 @@ val pp_term_def = tDefine "pp_term" `
     | Abs (Var _ _) r =>
         let (vs, b) = collect_vars tm in
         let ind = if prec = 0 then 4 else 5 in
-          (case vs of
-             [v] =>
-               pp_paren_blk ind (0 < prec)
-                   [mk_str (strlit"\\" ^ v ^ strlit".");
-                    mk_str space;
-                    pp_term 0 b]
-           | _ =>
              pp_paren_blk ind (0 < prec)
                ((mk_str (strlit"\\") :: pp_seq mk_str F space vs) ++
                 [mk_str (strlit".");
-                 mk_brk 1;
-                 pp_term 0 b]))
-    | Abs _ _ => mk_str (strlit"<bogus abstraction>")
+                 (if 1 < LENGTH vs then mk_brk 1 else mk_str space);
+                 pp_term 0 b])
+    | Abs _ _ => mk_str (strlit"<pp_term: bogus abstraction>")
     | Const n ty => mk_str (name_of n) (* Hide Data.Bool and Data.Pair *)
     | Var n ty => mk_str n)`
   (WF_REL_TAC `measure (term_size o SND)`
-   \\ rw [Once collect_vars_def, UNCURRY]
-   \\ fs [Once collect_vars_def]
+   \\ rw [Once collect_vars_def]
+   \\ fs [Once dest_binary_def, Once dest_binder_def] \\ rw []
+   \\ fs [is_binop_def, is_cond_def, is_binder_def, is_neg_def]
    \\ pairarg_tac \\ fs [] \\ rw []
-   \\ rename1 `collect_vars tm`
-   \\ `term_size (SND (collect_vars tm)) <= term_size tm` suffices_by rw []
-   \\ fs [collect_vars_term_size]);
+   >-
+    (rename1 `collect_vars tm` \\ fs []
+     \\ `term_size (SND (collect_vars tm)) <= term_size tm` suffices_by rw []
+     \\ fs [collect_vars_term_size])
+   \\ imp_res_tac dest_binary_MEM_term_size \\ fs []
+   >-
+    (rename1 `dest_binary nm tm`
+     \\ `term_size (SND (dest_binary nm tm)) <= term_size tm` suffices_by rw []
+     \\ fs [dest_binary_term_size])
+   \\ imp_res_tac dest_binder_term_size \\ fs []);
 
 (* ------------------------------------------------------------------------- *)
 (* A pretty printer for theorems.                                            *)
@@ -277,6 +396,96 @@ val term2str_def = Define `
 
 val thm2str_def = Define `
   thm2str thm = pr (pp_thm thm) pp_margin`;
+
+(* ------------------------------------------------------------------------- *)
+(* PMATCH definitions.                                                       *)
+(* ------------------------------------------------------------------------- *)
+
+val _ = patternMatchesLib.ENABLE_PMATCH_CASES ();
+val PMATCH_ELIM_CONV = patternMatchesLib.PMATCH_ELIM_CONV;
+
+val is_binop_PMATCH = Q.store_thm("is_binop_PMATCH",
+  `!tm.
+     is_binop tm =
+       case tm of
+         Comb (Comb (Const con _) _) _ =>
+           (case fixity_of con of
+              right _ => T
+            | _ => F)
+       | _ => F`,
+  CONV_TAC (DEPTH_CONV PMATCH_ELIM_CONV)
+  \\ simp [is_binop_def]);
+
+val is_binder_PMATCH = Q.store_thm("is_binder_PMATCH",
+  `!tm.
+     is_binder tm =
+       case tm of
+         Comb (Const nm _) (Abs (Var _ _) _) =>
+           nm = strlit"Data.Bool.?" \/
+           nm = strlit"Data.Bool.!" \/
+           nm = strlit"Data.Bool.?!" \/
+           nm = strlit"@"
+       | _ => F`,
+  CONV_TAC (DEPTH_CONV PMATCH_ELIM_CONV)
+  \\ simp [is_binder_def]);
+
+val is_cond_PMATCH = Q.store_thm("is_cond_PMATCH",
+  `!tm.
+     is_cond tm =
+       case tm of
+         Comb (Comb (Comb (Const con _) _) _) _ =>
+           con = strlit"Data.Bool.cond"
+       | _ => F`,
+  CONV_TAC (DEPTH_CONV PMATCH_ELIM_CONV)
+  \\ simp [is_cond_def]);
+
+val is_neg_PMATCH = Q.store_thm("is_neg_PMATCH",
+  `!tm.
+     is_neg tm =
+       case tm of
+         Comb (Const nm _) _ => nm = strlit"Data.Bool.~"
+       | _ => F`,
+  CONV_TAC (DEPTH_CONV PMATCH_ELIM_CONV)
+  \\ simp [is_neg_def]);
+
+val collect_vars_PMATCH = Q.store_thm("collect_vars_PMATCH",
+  `!tm.
+     collect_vars tm =
+       case tm of
+         Abs (Var v ty) r =>
+           let (vs, b) = collect_vars r in
+             (v::vs, b)
+       | _ => ([], tm)`,
+  CONV_TAC (DEPTH_CONV PMATCH_ELIM_CONV)
+  \\ simp [Once collect_vars_def]);
+
+val dest_binary_PMATCH = Q.store_thm("dest_binary_PMATCH",
+  `!tm.
+     dest_binary nm tm =
+       case tm of
+         Comb (Comb (Const nm' _) l) r =>
+           if nm <> nm' then
+             ([], tm)
+           else
+             let (ls, r) = dest_binary nm r in
+               (l::ls, r)
+       | _ => ([], tm)`,
+  CONV_TAC (DEPTH_CONV PMATCH_ELIM_CONV)
+  \\ simp [Once dest_binary_def]);
+
+val dest_binder_PMATCH = Q.store_thm("dest_binder_PMATCH",
+  `!tm.
+     dest_binder nm tm =
+       case tm of
+         Comb (Const nm' _) (Abs (Var v _) b) =>
+           if nm <> nm' then
+             ([], tm)
+           else
+             let (vs, r) = dest_binder nm b in
+               (v::vs, r)
+       | _ => ([], tm)`,
+  CONV_TAC (DEPTH_CONV PMATCH_ELIM_CONV)
+  \\ simp [Once dest_binder_def]);
 
 val _ = export_theory ();
 
